\documentclass{article}
\usepackage[margin=1in]{geometry}
\usepackage[utf8]{inputenc}
\usepackage{amsmath}
\usepackage{amsfonts}
\usepackage{amssymb}
\usepackage{graphicx}

\title{Homework 2}
\author{Giacomo Cappelletto}
\date{\today}

\begin{document}

\maketitle

\section{Linear Transformations}

\subsection*{A)}
\subsubsection*{I)}
\[
	\begin{bmatrix}
		2 & 0 \\
		0 & 2
	\end{bmatrix}
\]
\subsubsection*{II)}

$$Scalar Matrix$$

\subsection*{B)}

\subsubsection*{I}

\[
	\begin{bmatrix}
		1 & -1 \\
		0 & 1
	\end{bmatrix}
\]
\subsubsection*{II)}

$$Horizontal shear$$

\subsection*{C)}

\subsubsection*{I)}

\[
	\begin{bmatrix}
		\cos(270^\circ) & -\sin(270^\circ) \\
		\sin(270^\circ) & \cos(270^\circ)
	\end{bmatrix}
	=
	\begin{bmatrix}
		0  & 1 \\
		-1 & 0
	\end{bmatrix}
\]

\subsubsection*{II)}

$$Rotation Matrix$$

\subsection{E)}

\subsubsection*{I)}

\[
	\begin{bmatrix}
		\cos(180^\circ) & -\sin(180^\circ) \\
		\sin(180^\circ) & \cos(180^\circ)
	\end{bmatrix}
	=
	\begin{bmatrix}
		1 & 0  \\
		0 & -1
	\end{bmatrix}
\]

\subsubsection*{II)}

$$Reflection Matrix$$

\subsection{F)}

\subsubsection*{I)}

\[
	\begin{bmatrix}
		1 & 0 \\
		0 & 0
	\end{bmatrix}
\]

\subsubsection*{II)}

$$Projection (matrix)$$

\section{Rotations}

\subsection*{A)}




$$	\cos(\theta + \phi) = \frac{v_1}{r} \Rightarrow v_1 = r \cdot \cos(\theta + \phi) $$
$$
	v= \begin{bmatrix}
		r \cdot \cos(\theta + \phi) \\
		r \cdot \sin(\theta + \phi)
	\end{bmatrix}
$$


$$	\cos(\theta) = \frac{z_1}{r} \Rightarrow z_1 = r \cdot \cos(\theta) $$
$$
	z= \begin{bmatrix}
		r \cdot \cos(\phi) \\
		r \cdot \sin(\phi)
	\end{bmatrix}
$$
\subsection*{B)}


Since
$$
	\cos(\theta + \phi) = \cos(\theta) \cos(\phi) - \sin(\theta) \sin(\phi)
$$
Then
$$
	v_1 = r \cdot \cos(\theta + \phi) = r \cdot \cos(\theta) \cos(\phi) - r \cdot \sin(\theta) \sin(\phi)
$$
\subsection*{C)}
Given
\[
	z_1 = r \cdot \cos(\theta) ,
	z_2 = \cdot \sin(\theta)
\]
Then
\[
	v_1 = z_1 \cdot \cos(\theta) - z_2 \cdot \sin(\theta)
\]

\subsection*{D)}

\[
	v_1 = \begin{bmatrix}
		\cos(\theta) & -\sin(\theta) \\
	\end{bmatrix}
	\cdot
	\begin{bmatrix}
		z_1 \\
		z_2
	\end{bmatrix}
	=
	z_1 \cdot \cos(\theta) - z_2 \cdot \sin(\theta)
\]

\subsection*{E)}
Since
$$
	\sin(\theta + \phi) = \sin(\theta) \cos(\phi) + \cos(\theta) \sin(\phi)
$$
Then
$$
	v_2 = r \cdot \sin(\theta + \phi) = r \cdot \sin(\theta) \cos(\phi) + r \cdot \cos(\theta) \sin(\phi)
$$

\subsection*{F)}
Given
\[
	z_1 = r \cdot \cos(\theta) ,
	z_2 = \cdot \sin(\theta)
\]
Then
\[
	v_2 = z_1 \cdot \sin(\theta) + z_2 \cdot \cos(\theta)
\]
\subsection*{G)}

\[
	v_2 = \begin{bmatrix}
		\sin(\theta) & \cos(\theta) \\
	\end{bmatrix}
	\cdot
	\begin{bmatrix}
		z_1 \\
		z_2
	\end{bmatrix}
	=
	z_1 \cdot \sin(\theta) + z_2 \cdot \cos(\theta)
\]

\subsection*{H)}

\[
	v = \begin{bmatrix}
		v_1 \\
		v_2
	\end{bmatrix}
	=
	\begin{bmatrix}
		\cos(\theta) & - \sin(\theta) \\
		\sin(\theta) & \cos(\theta)
	\end{bmatrix}
	\cdot
	\begin{bmatrix}
		z_1 \\
		z_2
	\end{bmatrix}
\]
\end{document}